Fix proof Load FTLR

theories/ftlr/Load.v
@@ -19,7 +19,9 @@ Section fundamental.
   (* The necessary resources to close the region again, except for the points to predicate, which we will store separately
    The boolean bl can be used to keep track of whether or not we have applied a wp lemma *)
   Definition region_open_resources (P : D) (w : Word) (a pc_a : Addr) (f:bool) : iProp Σ :=
-    ((if f then ▷ P w else P w) ∗ read_cond P interp ∗ ((▷ ∃ w0, a ↦ₐ w0 ∗ P w0) ={⊤ ∖ ↑logN.@pc_a ∖ ↑logN.@a,⊤ ∖ ↑logN.@pc_a}=∗ emp))%I.
+    ((if f then ▷ P w else P w)
+       ∗ read_cond P interp
+       ∗ ((▷ ∃ w0, a ↦ₐ w0 ∗ P w0) ={⊤ ∖ ↑logN.@pc_a ∖ ↑logN.@a,⊤ ∖ ↑logN.@pc_a}=∗ emp))%I.
 
   Lemma load_inr_eq {regs r p0 b0 e0 a0 p1 b1 e1 a1}:
     reg_allows_load regs r p0 b0 e0 a0 →
@@ -33,70 +35,104 @@ Section fundamental.
 
 
   (* Description of what the resources are supposed to look like after opening the region if we need to, but before closing the region up again*)
-  Definition allow_load_res r (regs : Reg) pc_a a p b e (P : D) :=
+  Definition allow_load_res (regs : Reg) (r : RegName)
+    (pc_a : Addr) (p : Perm) (b e a : Addr) (P : D) :=
     (⌜read_reg_inr regs r p b e a⌝ ∗
-    if decide (reg_allows_load regs r p b e a ∧ a ≠ pc_a ) then
-         |={⊤ ∖ ↑logN.@pc_a,⊤ ∖ ↑logN.@pc_a ∖ ↑logN.@a}=> ∃ w, a ↦ₐ w ∗ region_open_resources P w a pc_a true ∗ ▷ interp w
-     else True)%I.
+       if decide (reg_allows_load regs r p b e a ∧ a ≠ pc_a )
+       then (|={⊤ ∖ ↑logN.@pc_a,⊤ ∖ ↑logN.@pc_a ∖ ↑logN.@a}=>
+              ∃ w, a ↦ₐ w ∗ region_open_resources P w a pc_a true ∗ ▷ interp w)
+       else True)%I.
 
-
-  Definition allow_load_mem r (regs : Reg) (pc_a : Addr) (pc_w : Word) (mem : gmap Addr Word) (a : Addr) p b e (P:D) (f:bool) :=
+  Definition allow_load_mem (regs : Reg) (mem : Mem) (r : RegName)
+    (pc_a : Addr) (pc_w : Word)
+    (p : Perm) (b e a : Addr)
+    (P:D) (f:bool) :=
     (⌜read_reg_inr regs r p b e a⌝ ∗
-    if decide (reg_allows_load regs r p b e a ∧ a ≠ pc_a) then
-         ∃ (w : Word), ⌜mem = <[a:=w]> (<[pc_a:=pc_w]> ∅)⌝ ∗
-            (region_open_resources P w a pc_a f) ∗ if f then ▷ interp w else interp w
-    else  ⌜mem = <[pc_a:=pc_w]> ∅⌝)%I.
+       if decide (reg_allows_load regs r p b e a ∧ a ≠ pc_a)
+       then ∃ (w : Word),
+           ⌜mem = <[a:=w]> (<[pc_a:=pc_w]> ∅)⌝
+           ∗ (region_open_resources P w a pc_a f)
+           ∗ if f then ▷ interp w else interp w
+       else  ⌜mem = <[pc_a:=pc_w]> ∅⌝)%I.
 
   Lemma create_load_res:
-    ∀ (r : leibnizO Reg) (p : Perm)
-      (b e a : Addr) (src : RegName) (p0 : Perm)
-      (b0 e0 a0 : Addr) (widc : Word),
-      read_reg_inr (<[PC:=WCap p b e a]> (<[idc:=widc]> r)) src p0 b0 e0 a0
-      → (∀ (r1 : RegName) v, ⌜r1 ≠ PC⌝ → ⌜r1 ≠ idc⌝ →⌜r !! r1 = Some v⌝ → (fixpoint interp1) v)
-          -∗ ∃ P, allow_load_res src (<[PC:=WCap p b e a]> (<[idc:=widc]> r)) a a0 p0 b0 e0 P.
+    ∀ (regs : leibnizO Reg) (src : RegName)
+      (pc_p : Perm) (pc_b pc_e pc_a : Addr)
+      (widc : Word)
+      (p : Perm) (b e a : Addr) ,
+      read_reg_inr (<[PC:=WCap pc_p pc_b pc_e pc_a]> (<[idc:=widc]> regs)) src p b e a
+      → (∀ (r : RegName) (w : Word), ⌜r ≠ PC⌝ → ⌜r ≠ idc⌝ → ⌜regs !! r = Some w⌝ → (fixpoint interp1) w)
+          -∗ interp widc
+          -∗ ∃ P, allow_load_res
+                    (<[PC:=WCap pc_p pc_b pc_e pc_a]> (<[idc:=widc]> regs))
+                    src pc_a p b e a P.
   Proof.
-    intros r p b e a src p0 b0 e0 a0 widc HVsrc.
-    iIntros "#Hreg". rewrite /allow_load_res.
+    intros regs src pc_p pc_b pc_e pc_a widc p b e a HVsrc.
+    iIntros "#Hreg #Hwidc". rewrite /allow_load_res.
     (* do 5 (iApply sep_exist_r; iExists _). *) (* do 3 (iExists _). *) iFrame "%".
     case_decide as Hdec. 1: destruct Hdec as [Hallows Haeq].
     -  destruct Hallows as [Hrinr [Hra Hwb] ].
          apply andb_prop in Hwb as [Hle Hge].
 
-         (* Unlike in the old proof, we now go the other way around, and prove that the source register could not have been the PC, since both addresses differ. This saves us some cases.*)
+         (* Unlike in the old proof, we now go the other way around,
+            and prove that the source register could not have been the PC,
+            since both addresses differ. This saves us some cases.*)
          assert (src ≠ PC) as n. refine (addr_ne_reg_ne Hrinr _ Haeq). by rewrite lookup_insert.
 
          rewrite lookup_insert_ne in Hrinr; last by congruence.
-         iDestruct ("Hreg" $! src _ n _ Hrinr) as "Hvsrc".
-         iDestruct (read_allowed_inv _ a0 with "Hvsrc") as (P) "[Hinv [Hpers [Hconds _]] ]"; auto;
+         destruct (decide (src = idc)) as [|Hneq]; simplify_map_eq.
+         + (* src = idc *)
+           iDestruct (read_allowed_inv _ a with "Hwidc") as (P) "[Hinv [Hpers [Hconds _]] ]"; auto;
+             first (split; [by apply Z.leb_le | by apply Z.ltb_lt]).
+           iExists P.
+           iMod (inv_acc (⊤ ∖ ↑logN.@pc_a) with "Hinv") as "[Hrefinv Hcls]";[solve_ndisj|].
+           rewrite /interp_ref_inv /=. iDestruct "Hrefinv" as (w) "[>Ha HP]".
+           iExists w.
+
+           iAssert (▷ interp w)%I as "#Hw".
+           { iNext. iApply "Hconds". iFrame. }
+           by iFrame "∗ #".
+
+         + (* src ≠ idc *)
+         iDestruct ("Hreg" $! src _ n Hneq Hrinr) as "Hvsrc".
+         iDestruct (read_allowed_inv _ a with "Hvsrc") as (P) "[Hinv [Hpers [Hconds _]] ]"; auto;
            first (split; [by apply Z.leb_le | by apply Z.ltb_lt]).
          iExists P.
-         iMod (inv_acc (⊤ ∖ ↑logN.@a) with "Hinv") as "[Hrefinv Hcls]";[solve_ndisj|].
+         iMod (inv_acc (⊤ ∖ ↑logN.@pc_a) with "Hinv") as "[Hrefinv Hcls]";[solve_ndisj|].
          rewrite /interp_ref_inv /=. iDestruct "Hrefinv" as (w) "[>Ha HP]".
          iExists w.
+
          iAssert (▷ interp w)%I as "#Hw".
          { iNext. iApply "Hconds". iFrame. }
-         iFrame "∗ #". iModIntro. rewrite /region_open_resources. done.
-    - iExists (λne _, True%I). done.
+         iFrame.
+         by iFrame "∗ #".
+    - by iExists (λne _, True%I).
   Qed.
 
-  (* Definition allow_load_mask (a a0 : Addr) : namespace := *)
-  (*   if decide (a = a0) then ⊤ ∖ ↑logN.@a else ⊤ ∖ ↑logN.@a ∖ ↑logN.@a0.  *)
+  Definition allow_load_mask (regs : Reg) (r : RegName)
+    (pc_a : Addr) (p : Perm) (b e a : Addr) : coPset :=
+    if decide (reg_allows_load regs r p b e a ∧ a ≠ pc_a)
+    then ⊤ ∖ ↑logN.@pc_a ∖ ↑logN.@a
+    else ⊤ ∖ ↑logN.@pc_a.
 
   Lemma load_res_implies_mem_map:
-    ∀ (r : leibnizO Reg)
-       (a a0 : Addr) (w : Word) (src : RegName) p1 b1 e1 (P:D),
-      allow_load_res src r a a0 p1 b1 e1 P
-      -∗ a ↦ₐ w
-      ={⊤ ∖ ↑logN.@a,if decide (reg_allows_load r src p1 b1 e1 a0 ∧ a0 ≠ a) then ⊤ ∖ ↑logN.@a ∖ ↑logN.@a0 else ⊤ ∖ ↑logN.@a}=∗ ∃ mem0 : gmap Addr Word,
-          allow_load_mem src r a w mem0 a0 p1 b1 e1 P true
-            ∗ ▷ ([∗ map] a0↦w ∈ mem0, a0 ↦ₐ w).
+    ∀ (regs : leibnizO Reg) (src : RegName)
+      (pc_a : Addr) (pc_w : Word)
+      (p : Perm) (b e a: Addr)  (P:D),
+      allow_load_res regs src pc_a p b e a P
+      -∗ pc_a ↦ₐ pc_w
+      ={⊤ ∖ ↑logN.@pc_a, allow_load_mask regs src pc_a p b e a}=∗ ∃ mem : Mem,
+          allow_load_mem regs mem src pc_a pc_w p b e a P true
+            ∗ ▷ ([∗ map] a0↦w ∈ mem, a0 ↦ₐ w).
   Proof.
-    intros r a a0 w src p1 b1 e1 P.
+    intros regs src pc_a pc_w p b e a P.
     iIntros "HLoadRes Ha".
     iDestruct "HLoadRes" as "[% HLoadRes]".
+    rewrite /allow_load_mask.
 
     case_decide as Hdec. 1: destruct Hdec as [ Hallows Haeq ].
-    -  pose(Hallows' := Hallows). destruct Hallows' as [Hrinr [Hra Hwb] ].
+    -  pose(Hallows' := Hallows).
+       destruct Hallows' as [Hrinr [Hra Hwb] ].
        iMod "HLoadRes" as (w0) "[Ha0 [HLoadRest #Hval] ]".
        iExists _.
        iSplitL "HLoadRest".
@@ -116,66 +152,77 @@ Section fundamental.
   Qed.
 
   Lemma mem_map_implies_pure_conds:
-    ∀ (r : leibnizO Reg)
-       (a a0 : Addr) (w : Word) (src : RegName)
-      (mem0 : gmap Addr Word) p b e P f,
-        allow_load_mem src r a w mem0 a0 p b e P f
-        -∗ ⌜mem0 !! a = Some w⌝
-          ∗ ⌜allow_load_map_or_true src r mem0⌝.
+    ∀ (regs : leibnizO Reg) (mem : Mem) (src : RegName)
+      (pc_a : Addr) (pc_w : Word)
+      (p : Perm) (b e a : Addr) (P : D) (f : bool),
+      allow_load_mem regs mem src pc_a pc_w p b e a P f
+        -∗ ⌜mem !! pc_a = Some pc_w⌝
+          ∗ ⌜allow_load_map_or_true src regs mem⌝.
   Proof.
-    iIntros (r a a0 w src mem0 p b e P f) "HLoadMem".
+    iIntros (regs mem src pc_a pc_w p b e a P f) "HLoadMem".
     iDestruct "HLoadMem" as "[% HLoadRes]".
     case_decide as Hdec. 1: destruct Hdec as [ Hallows Haeq ].
     -  pose(Hallows' := Hallows). destruct Hallows' as [Hrinr [Hra Hwb] ].
-       (* case_decide as Haeq. *)
-       iDestruct "HLoadRes" as (w0) "[% _]".
-       iSplitR. rewrite H1 lookup_insert_ne; auto. by rewrite lookup_insert.
-       iExists p,b,e,a0. iSplitR; auto.
+       iDestruct "HLoadRes" as (w0) "[%Hmem _]".
+       iSplitR. rewrite Hmem lookup_insert_ne; auto. by rewrite lookup_insert.
+       iExists p,b,e,a. iSplitR; auto.
        case_decide; last by exfalso.
-       iExists w0. rewrite H1.
-         by rewrite lookup_insert.
+       iExists w0. rewrite Hmem. by rewrite lookup_insert.
     - iDestruct "HLoadRes" as "->".
       iSplitR. by rewrite lookup_insert.
-      iExists p,b,e,a0. iSplitR; auto.
+      iExists p,b,e,a. iSplitR; auto.
       case_decide as Hdec1; last by done.
       apply not_and_r in Hdec as [| <-%dec_stable]; first by exfalso.
-      iExists w. by rewrite lookup_insert.
+      iExists pc_w. by rewrite lookup_insert.
   Qed.
 
   Lemma allow_load_mem_later:
-    ∀ (r : leibnizO Reg) (p : Perm)
-      (b e a a0 : Addr) (w : Word) (src : RegName)
-      (mem0 : gmap Addr Word) p0 b0 e0 P,
-      allow_load_mem src r a w mem0 a0 p0 b0 e0 P true
-      -∗ ▷ allow_load_mem src r a w mem0 a0 p0 b0 e0 P false.
+    ∀ (regs : leibnizO Reg) (mem : Mem) (src : RegName)
+      (pc_p : Perm) (pc_b pc_e pc_a : Addr) (pc_w : Word)
+      (p : Perm) (b e a : Addr) (P : D),
+      allow_load_mem regs mem src pc_a pc_w p b e a P true
+      -∗ ▷ allow_load_mem regs mem src pc_a pc_w p b e a P false.
   Proof.
-    iIntros (r p b e a a0 w src mem0 p0 b0 e0 P) "HLoadMem".
+    iIntros (regs mem src pc_p pc_b pc_e pc_a pc_w p b e a P) "HLoadMem".
     iDestruct "HLoadMem" as "[% HLoadMem]".
     rewrite !/allow_load_mem /=. iSplit;[auto|].
-    destruct (decide (reg_allows_load r src p0 b0 e0 a0 ∧ a0 ≠ a)).
+    destruct (decide (reg_allows_load regs src p b e a ∧ a ≠ pc_a)).
     - iApply later_exist_2. iDestruct "HLoadMem" as (w0) "(?&HP&?)".
       iExists w0. iNext. iDestruct "HP" as "(?&?&?)". iFrame.
     - iNext. iFrame.
   Qed.
 
-  Instance if_Persistent p b e a r src p0 b0 e0 a0 loadv : Persistent (if decide (reg_allows_load (<[PC:=WCap p b e a]> r) src p0 b0 e0 a0 ∧ a0 ≠ a) then interp loadv else emp)%I.
-  Proof. intros. destruct (decide (reg_allows_load (<[PC:=WCap p b e a]> r) src p0 b0 e0 a0 ∧ a0 ≠ a));apply _. Qed.
+  Instance if_Persistent
+    (regs : Reg) (src : RegName)
+    (pc_p : Perm) (pc_b pc_e pc_a : Addr)
+    (p : Perm) (b e a : Addr) (loadv : Word) :
+    Persistent
+      (if decide (reg_allows_load (<[PC:=WCap pc_p pc_b pc_e pc_a]> regs) src p b e a ∧ a ≠ pc_a)
+       then interp loadv
+       else emp)%I.
+  Proof. intros.
+         destruct (decide (reg_allows_load (<[PC:=WCap pc_p pc_b pc_e pc_a]> regs)
+                             src p b e a ∧ a ≠ pc_a)); apply _.
+  Qed.
 
   Lemma mem_map_recover_res:
-    ∀ (r : leibnizO Reg)
-       (a : Addr) (w : Word) (src : RegName) p0
-       (b0 e0 a0 : Addr) (mem0 : gmap Addr Word) loadv P,
-      mem0 !! a0 = Some loadv
-      -> reg_allows_load r src p0 b0 e0 a0
-      → allow_load_mem src r a w mem0 a0 p0 b0 e0 P false
-        -∗ ([∗ map] a0↦w ∈ mem0, a0 ↦ₐ w)
-        ={if decide (reg_allows_load r src p0 b0 e0 a0 ∧ a0 ≠ a) then ⊤ ∖ ↑logN.@a ∖ ↑logN.@a0 else ⊤ ∖ ↑logN.@a,⊤ ∖ ↑logN.@a}=∗ a ↦ₐ w
-                  ∗ if decide (reg_allows_load r src p0 b0 e0 a0 ∧ a0 ≠ a) then interp loadv else emp.
+    ∀ (regs : leibnizO Reg) (mem : Mem) (src : RegName)
+       (pc_a : Addr) (pc_w : Word)
+       (p : Perm) (b e a : Addr) (loadv : Word) (P : D),
+      mem !! a = Some loadv
+      -> reg_allows_load regs src p b e a
+      → allow_load_mem regs mem src pc_a pc_w p b e a P false
+        -∗ ([∗ map] a↦w ∈ mem, a ↦ₐ w)
+        ={allow_load_mask regs src pc_a p b e a,⊤ ∖ ↑logN.@pc_a}=∗
+        pc_a ↦ₐ pc_w ∗
+        if decide (reg_allows_load regs src p b e a ∧ a ≠ pc_a)
+        then interp loadv
+        else emp.
   Proof.
-    intros r a w src p0 b0 e0 a0 mem0 loadv P Hloadv Hrar.
+    intros regs mem src pc_a pc_w p b e a loadv P Hloadv Hrar.
     iIntros "HLoadMem Hmem".
+    rewrite /allow_load_mask.
     iDestruct "HLoadMem" as "[% HLoadRes]".
-    (* destruct (load_inr_eq Hrar H0) as (<- & <- &<- &<- &<-). *)
     case_decide as Hdec. destruct Hdec as [Hallows Heq].
     -  destruct Hallows as [Hrinr [Hra Hwb] ].
        iDestruct "HLoadRes" as (w0) "[-> [ [HP [#Hcond Hcls] ] Hinterp] ]".
@@ -188,10 +235,9 @@ Section fundamental.
         rewrite -memMap_resource_1. by iFrame.
   Qed.
 
-
-  Lemma load_case (r : leibnizO Reg) (p : Perm)
+  Lemma load_case (regs : leibnizO Reg) (p : Perm)
         (b e a : Addr) (widc w : Word) (dst src : RegName) (P : D):
-    ftlr_instr r p b e a widc w (Load dst src) P.
+    ftlr_instr regs p b e a widc w (Load dst src) P.
   Proof.
     intros Hp Hsome i Hbae Hi.
     iIntros
@@ -199,7 +245,7 @@ Section fundamental.
     iInsertList "Hmap" [idc;PC].
 
     (* To read out PC's name later, and needed when calling wp_load *)
-    assert(∀ x : RegName, is_Some (<[PC:=WCap p b e a]> (<[idc:=widc]> r) !! x)) as Hsome'.
+    assert(∀ x : RegName, is_Some (<[PC:=WCap p b e a]> (<[idc:=widc]> regs) !! x)) as Hsome'.
     {
       intros. destruct (decide (x = PC)).
       rewrite e0 lookup_insert; unfold is_Some. by eexists.
@@ -210,7 +256,7 @@ Section fundamental.
     }
 
     (* Initializing the names for the values of Hsrc now, to instantiate the existentials in step 1 *)
-    assert (∃ p0 b0 e0 a0, read_reg_inr (<[PC:=WCap p b e a]> (<[idc:=widc]> r)) src p0 b0 e0 a0)
+    assert (∃ p0 b0 e0 a0, read_reg_inr (<[PC:=WCap p b e a]> (<[idc:=widc]> regs)) src p0 b0 e0 a0)
       as [p0 [b0 [e0 [a0 HVsrc] ] ] ].
     {
       specialize Hsome' with src as Hsrc.
@@ -220,11 +266,12 @@ Section fundamental.
       by repeat eexists.
     }
 
+    (* Step 1: open the region, if necessary, and store all the resources
+       obtained from the region in allow_load_res *)
+    iDestruct (create_load_res with "Hreg Hinv_idc") as (P') "HLoadRes"; eauto.
 
-    (* Step 1: open the region, if necessary, and store all the resources obtained from the region in allow_load_res *)
-    iDestruct (create_load_res with "Hreg") as (P') "HLoadRes"; eauto.
-
-    (* Step2: derive the concrete map of memory we need, and any spatial predicates holding over it *)
+    (* Step2: derive the concrete map of memory we need, and any spatial
+       predicates holding over it *)
     iMod (load_res_implies_mem_map with "HLoadRes Ha") as (mem0) "[HLoadMem HLoadRest]".
 
     (* Step 3:  derive the non-spatial conditions over the memory map*)
@@ -236,27 +283,27 @@ Section fundamental.
     iApply (wp_load with "[Hmap HLoadRest]");eauto.
     { by rewrite lookup_insert. }
     { rewrite /subseteq /map_subseteq /set_subseteq_instance. intros rr _.
-      apply elem_of_dom. rewrite lookup_insert_is_Some'; eauto. }
+      apply elem_of_dom. repeat (rewrite lookup_insert_is_Some'; right); eauto. }
     { iSplitR "Hmap"; auto. }
     iNext. iIntros (regs' retv). iDestruct 1 as (HSpec) "[Hmem Hmap]".
 
     (* Infer that if P holds at w, then w must be valid (read condition) *)
     iDestruct ("Hread" with "HP") as "#Hw".
 
-    destruct HSpec as [* ? ? Hincr|].
-    { apply incrementPC_Some_inv in Hincr.
-      destruct Hincr as (?&?&?&?&?&?&?&?).
+    destruct HSpec as [* Hrallows Hmem HincrPC|].
+    { apply incrementPC_Some_inv in HincrPC as (p''&b''&e''&a''& ? & HPC & Z & Hregs') .
       iApply wp_pure_step_later; auto.
-      specialize (load_inr_eq H0 HVsrc) as (-> & -> & -> & ->).
+      specialize (load_inr_eq Hrallows HVsrc) as (-> & -> & -> & ->).
       rewrite /allow_load_res.
       (* Step 5: return all the resources we had in order to close the second location in the region, in the cases where we need to *)
       iMod (mem_map_recover_res with "HLoadMem Hmem") as "[Ha #Hinterp]";[eauto|auto|iModIntro].
       iMod ("Hcls" with "[Ha HP]");[iExists w;iFrame|iModIntro].
 
-      (* Exceptional success case: we do not apply the induction hypothesis in case we have a faulty PC *)
-      destruct (decide (x = RX ∨ x = RWX)).
+      (* Exceptional success case: we do not apply the induction hypothesis in case
+         we have a faulty PC *)
+      destruct (decide (p'' = RX ∨ p'' = RWX)).
       2 : {
-        assert (x ≠ RX ∧ x ≠ RWX). split; by auto.
+        assert (p'' ≠ RX ∧ p'' ≠ RWX). split; by auto.
         iDestruct ((big_sepM_delete _ _ PC) with "Hmap") as "[HPC Hmap]".
         { subst. by rewrite lookup_insert. }
         iNext; iIntros "_".
@@ -268,44 +315,69 @@ Section fundamental.
         iIntros (a1); inversion a1.
       }
 
+      set (widc' := if (decide (dst = idc))
+                    then loadv
+                    else widc).
       iNext; iIntros "_".
-      iApply ("IH" $! regs' with "[%] [Hinterp] [Hmap] [$Hown]").
-      { cbn. intros. subst regs'.
-        rewrite lookup_insert_is_Some.
-        destruct (decide (PC = x4)); [ auto | right; split; auto].
-        rewrite lookup_insert_is_Some.
-        destruct (decide (dst = x4)); [ auto | right; split; auto]. }
-      (* Prove in the general case that the value relation holds for the register that was loaded to - unless it was the PC.*)
-       { iIntros (ri v Hri Hvs).
-        subst regs'.
-        rewrite lookup_insert_ne in Hvs; auto.
-        destruct (decide (ri = dst)).
-        { subst ri.
-          rewrite lookup_insert in Hvs; auto. inversion Hvs.
-          destruct (decide (a = a0)).
-          - simplify_eq. iFrame "Hw".
-          - iClear "HLoadRes Hwrite". rewrite decide_True. iFrame "#". auto.
+      iApply ("IH" $! regs' _ _ _ _ widc' with "[%] [Hinterp] [Hmap] [$Hown]"); subst regs'.
+      { intro; cbn; by repeat (rewrite lookup_insert_is_Some'; right). }
+      (* Prove in the general case that the value relation holds for the register
+         that was loaded to - unless it was the PC.*)
+      { iIntros (ri v Hri Hri' Hvs).
+        destruct (decide (ri = dst)); simplify_map_eq.
+        { destruct (decide (a0 = a'')); simplify_eq.
+          - rewrite HReadPC in Hmem; simplify_eq. iFrame "Hw".
+          - iClear "HLoadRes Hwrite". rewrite decide_True; auto.
         }
         { repeat (rewrite lookup_insert_ne in Hvs); auto.
           iApply "Hreg"; auto. }
-       }
-       { subst regs'. rewrite insert_insert. iApply "Hmap". }
-       { iModIntro.
-         destruct (decide (PC = dst)); simplify_eq.
-         - simplify_map_eq. rewrite (fixpoint_interp1_eq).
-           destruct (decide (a = a0)).
-           + simplify_map_eq.
-           + iClear "HLoadRes Hwrite". rewrite decide_True;auto.
-             rewrite !fixpoint_interp1_eq.
-             destruct o as [-> | ->]; iFrame "Hinterp".
-         - (* iExists p'. *) simplify_map_eq.
-           iClear "Hw Hinterp Hwrite".
-           rewrite !fixpoint_interp1_eq /=.
-           destruct o as [-> | ->]; iFrame "Hinv".
-       }
+      }
+      { subst widc'.
+        iClear "Hwrite Hinterp".
+        destruct (decide (dst = idc)); simplify_map_eq.
+        + rewrite
+            (insert_commute _ idc _ loadv) //=
+            !insert_insert
+            (insert_commute _ idc _ loadv) //=
+            !insert_insert ; iFrame.
+        + destruct (decide (dst = PC)); simplify_map_eq.
+          * rewrite
+              !insert_insert
+              (insert_commute _ idc _ ) //=
+              insert_insert; iFrame.
+          * rewrite
+              (insert_commute _ PC _ ) //=
+              !insert_insert
+              (insert_commute _ idc) //=
+              (insert_commute _ idc) //=
+              (insert_commute _ idc) //=
+              (insert_commute _ idc) //=
+              insert_insert; iFrame.
+      }
+      { iModIntro.
+        destruct (decide (PC = dst)); simplify_eq.
+        - simplify_map_eq. rewrite (fixpoint_interp1_eq).
+          destruct (decide (a0 = a)); simplify_eq.
+          + rewrite HReadPC in Hmem; simplify_eq.
+          + iClear "HLoadRes Hwrite". rewrite decide_True;auto.
+            rewrite !fixpoint_interp1_eq.
+            destruct o as [-> | ->]; iFrame "Hinterp".
+        - simplify_map_eq.
+          iClear "Hw Hinterp Hwrite".
+          rewrite !fixpoint_interp1_eq /=.
+          destruct o as [-> | ->]; iFrame "Hinv_pc".
+      }
+      { iClear "Hwrite".
+        subst widc'. destruct (decide (dst = idc)); auto; simplify_map_eq.
+        destruct (decide (a0 = a'')); simplify_eq.
+        + by rewrite HReadPC in Hmem; simplify_eq.
+        + case_decide as Hcontra; auto.
+          exfalso ; apply Hcontra ; split; auto.
+      }
     }
-    { rewrite /allow_load_res /allow_load_mem.
-      destruct (decide (reg_allows_load (<[PC:=WCap p b e a]> r) src p0 b0 e0 a0 ∧ a0 ≠ a)).
+
+    { rewrite /allow_load_res /allow_load_mem /allow_load_mask.
+      destruct (decide (reg_allows_load (<[PC:=WCap p b e a]> (<[idc:=widc]> regs)) src p0 b0 e0 a0 ∧ a0 ≠ a)).
       - iDestruct "HLoadMem" as "(_&H)".
         iDestruct "H" as (w') "(->&Hres&Hinterp)". rewrite /region_open_resources.
         destruct a1. rewrite memMap_resource_2ne; last auto.
